theory/JITPer_call.thy
@@ -159,21 +159,24 @@ proof-
     by (simp add: per_jit_call_reg_def) 
 
 
-  have "l = x64_encode (Pcall_i 0)" using per_jit_call_reg_def c3_0 by simp
+  have c4_2:"l = x64_encode (Pcall_i 0)" using per_jit_call_reg_def c3_0 by simp
   hence c4_0:"off = ucast imm" using per_jit_call_reg_def c3_0 by simp
 
   have c4:"(l!0 = 0xe8)" using c_aux c3 c3_0 apply(unfold per_jit_call_reg_def x64_encode_def)
     apply(cases "Pcall_i (ucast imm)",simp_all) 
     subgoal for x16 by auto[1]
     done
-  have c4_1:"l!0 \<noteq> 0xc3" using c4 by simp
+  have "length l = 5" using c4_2 apply(unfold x64_encode_def Let_def,simp_all) apply(unfold u8_list_of_u32_def,simp_all) done
+  hence c4_1:"x64_decode 0 l = Some (5,Pcall_i 0)" using c4 c4_2 x64_encode_decode_consistency list_in_list_prop by blast
+  hence c4_3:"x64_decode 0 l \<noteq> Some(1,Pret)" by simp
   have c5:"?perir_step = (let caller = save_x64_caller xrs; fp = save_x64_frame_pointer xrs;
                            xrs' = upate_x64_stack_pointer xrs (stack_pointer xss) in
             let ss' = update_stack caller fp (pc+1) xss in
               (case ss' of None \<Rightarrow> (pc, Stuck) | 
               Some ra \<Rightarrow> (off, Next xpc xrs' xm ra)))" 
-    using c4 c2_1 perir_step_def a3 c_aux c_aux c4_1
-    by (smt (z3) One_nat_def case_prod_conv fst_conv option.case_eq_if outcome.simps(4) snd_conv perir_sem.simps(1) perir_sem.simps(2)) 
+    using c4 c2_1 perir_step_def a3 c_aux c_aux c4_1 c4_3
+    by (smt (verit) One_nat_def case_prod_conv fst_conv option.case_eq_if outcome.simps(4) perir_sem.simps(1) perir_sem.simps(2) snd_conv) 
+    
 
   have d1_1:"xss = ss" using match_state_def a0 a1 a2 a3 a4 by auto
   have d2_0:"call_depth xss +1 \<noteq>  max_call_depth" using c5 update_stack_def call_reg_subgoal_aux3 a0 a1 a2 a6 d1_1 using a8 by auto
